Examples/Examples.dfy
@@ -15,13 +15,23 @@ module RandomExamples {
   {
     var r := new DRandom();
 
+    print "Coin(): \n";
     for i := 0 to 20 {
       var b := r.Coin();
       print b, "\n";
     }
+  
+    print "\n";
+
+    print "UniformPowerOfTwo(3): \n";
+    for i := 0 to 20 {
+      var u := r.UniformPowerOfTwo(3);
+      print u, "\n";
+    }
 
     print "\n";
 
+    print "Uniform(10): \n";
     for i := 0 to 20 {
       var u := r.Uniform(10);
       print u, "\n";
@@ -29,6 +39,7 @@ module RandomExamples {
 
     print "\n";
 
+    print "UniformInterval(3,6): \n";
     for i := 0 to 20 {
       var u := r.UniformInterval(3, 6);
       print u, "\n";
@@ -36,6 +47,7 @@ module RandomExamples {
 
     print "\n";
 
+    print "Geometric(): \n";
     for i := 0 to 20 {
       var u := r.Geometric();
       print u, "\n";
@@ -43,6 +55,7 @@ module RandomExamples {
 
     print "\n";
 
+    print "Bernoulli(): \n";
     for i := 0 to 20 {
       var u := r.Bernoulli(0.2);
       print u, "\n";
