Library/DRandom.dfy
@@ -25,12 +25,19 @@ module {:extern "DafnyLibraries"} DafnyLibraries {
       modifies this
       ensures CoinModel(old(s)) == (b, s)
 
+    // 0 <= u < n
+    method UniformPowerOfTwo(n: nat) returns (u: nat)
+      modifies this
+      ensures UniformPowerOfTwoModel(n)(old(s)) == (u, s)
+
+    // 0 <= u < n
     method Uniform(n: nat) returns (u: nat)
       modifies this
       decreases *
       requires 0 < n
       ensures UniformModel(n)(old(s)) == (u, s)
 
+    // a <= u < b
     method UniformInterval(a: int, b: int) returns (u: int)
       modifies this
       decreases *
@@ -58,6 +65,32 @@ module {:extern "DafnyLibraries"} DafnyLibraries {
       modifies this
       ensures CoinModel(old(s)) == (b, s)   
 
+    method UniformPowerOfTwo(n: nat) returns (u: nat)
+      modifies this
+      ensures UniformPowerOfTwoModel(n)(old(s)) == (u, s)
+    {
+      var k := 1;
+      u := 0;
+
+      if k <= n {
+        var b := Coin();
+        k := 2*k;
+        u := if b then 2*u + 1 else 2*u;
+      }
+
+      while k <= n
+        decreases 2*n - k
+        invariant k >= 1
+        invariant UniformPowerOfTwoModel(n)(old(s)) == UniformPowerOfTwoModel(n, k, u)(s)
+      {
+        var b := Coin();
+        k := 2*k;
+        u := if b then 2*u + 1 else 2*u;
+      }
+    }
+
+
+
     // Based on https://arxiv.org/pdf/1304.1916.pdf; unverified.
     method Uniform(n: nat) returns (u: nat)
       modifies this
@@ -65,6 +98,14 @@ module {:extern "DafnyLibraries"} DafnyLibraries {
       requires n > 0
       ensures UniformModel(n)(old(s)) == (u, s)
     {
+/*       u := UniformPowerOfTwo(n-1);
+      while u >= n
+        decreases *
+        invariant UniformModel(n)(old(s)) == UniformPowerOfTwoModel(n-1)(old(s))
+        invariant (u, s) == UniformPowerOfTwoModel(n-1)(old(s))
+      {
+        u := UniformPowerOfTwo(n-1);
+      } */
       assume {:axiom} false;
       var v := 1;
       u := 0;
